RocqOfRust/core/links/borrow.v
@@ -12,18 +12,25 @@ where
 }
 *)
 Module Borrow.
-  Definition trait (Self Borrowed : Set) `{Link Self} `{Link Borrowed} : TraitMethod.Header.t :=
-    ("core::borrow::Borrow", [], [ Φ Borrowed ], Φ Self).
+  Definition trait (Self Borrowed : Set) `{Link Self} `{Link Borrowed} : TraitHeader.t :=
+    {|
+      TraitHeader.trait_name := "core::borrow::Borrow";
+      TraitHeader.trait_consts := [];
+      TraitHeader.trait_tys := [ Φ Borrowed ];
+      TraitHeader.self_ty := Φ Self;
+    |}.
 
-  Definition Run_borrow (Self Borrowed : Set) `{Link Self} `{Link Borrowed} : Set :=
-    TraitMethod.C (trait Self Borrowed) "borrow" (fun method =>
-      forall (self : '& Self),
-      Run.Trait method [] [] [ φ self ] ('& Borrowed)).
+  Class Method_borrow (Self Borrowed : Set) `{Link Self} `{Link Borrowed} : Set := {
+    borrow : PolymorphicFunction.t;
+    borrow_is_method :: IsTraitMethod.C (trait Self Borrowed) "borrow" borrow;
+    run_borrow (self : '& Self) :: Run.Trait borrow [] [] [ φ self ] ('& Borrowed);
+  }.
 
   Class Run (Self Borrowed : Set) `{Link Self} `{Link Borrowed} : Set := {
-    borrow : Run_borrow Self Borrowed;
+    method_borrow :: Method_borrow Self Borrowed;
   }.
 End Borrow.
+Export (hints) Borrow.
 
 (* impl<T: ?Sized> Borrow<T> for T *)
 Module Impl_Borrow_T_for_T.
@@ -41,16 +48,23 @@ pub trait BorrowMut<Borrowed: ?Sized>: Borrow<Borrowed> {
 }
 *)
 Module BorrowMut.
-  Definition trait (Self Borrowed : Set) `{Link Self} `{Link Borrowed} : TraitMethod.Header.t :=
-    ("core::borrow::BorrowMut", [], [ Φ Borrowed ], Φ Self).
+  Definition trait (Self Borrowed : Set) `{Link Self} `{Link Borrowed} : TraitHeader.t :=
+    {|
+      TraitHeader.trait_name := "core::borrow::BorrowMut";
+      TraitHeader.trait_consts := [];
+      TraitHeader.trait_tys := [ Φ Borrowed ];
+      TraitHeader.self_ty := Φ Self;
+    |}.
 
-  Definition Run_borrow_mut (Self Borrowed : Set) `{Link Self} `{Link Borrowed} : Set :=
-    TraitMethod.C (trait Self Borrowed) "borrow_mut" (fun method =>
-      forall (self : '&mut Self),
-      Run.Trait method [] [] [ φ self ] ('&mut Borrowed)).
+  Class Method_borrow_mut (Self Borrowed : Set) `{Link Self} `{Link Borrowed} : Set := {
+    borrow_mut : PolymorphicFunction.t;
+    borrow_mut_is_method :: IsTraitMethod.C (trait Self Borrowed) "borrow_mut" borrow_mut;
+    run_borrow_mut (self : '&mut Self) :: Run.Trait borrow_mut [] [] [ φ self ] ('&mut Borrowed);
+  }.
 
   Class Run (Self Borrowed : Set) `{Link Self} `{Link Borrowed} : Set := {
     run_Borrow_for_Self : Borrow.Run Self Borrowed;
-    borrow_mut : Run_borrow_mut Self Borrowed;
+    method_borrow_mut :: Method_borrow_mut Self Borrowed;
   }.
 End BorrowMut.
+Export (hints) BorrowMut.
