RocqOfRust/ruint/links/from.v
@@ -57,19 +57,25 @@ Export (hints) ToUintError.
   }
 *)
 Module UintTryFrom.
-  Definition trait (Self T : Set) `{Link Self} `{Link T} : TraitMethod.Header.t :=
-    ("ruint::from::UintTryFrom", [], [Φ T], Φ Self).
+  Definition trait (Self T : Set) `{Link Self} `{Link T} : TraitHeader.t :=
+    {|
+      TraitHeader.trait_name := "ruint::from::UintTryFrom";
+      TraitHeader.trait_consts := [];
+      TraitHeader.trait_tys := [Φ T];
+      TraitHeader.self_ty := Φ Self;
+    |}.
 
-  Definition Run_uint_try_from (Self T : Set) `{Link Self} `{Link T} : Set :=
-    TraitMethod.C (trait Self T) "uint_try_from" (fun method =>
-      forall (value : T),
-      Run.Trait method [] [] [ φ value ] (Result.t Self (ToUintError.t Self))
-    ).
+  Class Method_uint_try_from (Self T : Set) `{Link Self} `{Link T} : Set := {
+    uint_try_from : PolymorphicFunction.t;
+    uint_try_from_is_method :: IsTraitMethod.C (trait Self T) "uint_try_from" uint_try_from;
+    run_uint_try_from (value : T) :: Run.Trait uint_try_from [] [] [ φ value ] (Result.t Self (ToUintError.t Self));
+  }.
 
   Class Run (Self : Set) (T : Set) `{Link Self} `{Link T} : Set := {
-    run_uint_try_from : Run_uint_try_from Self T;
+    method_uint_try_from :: Method_uint_try_from Self T;
   }.
 End UintTryFrom.
+Export (hints) UintTryFrom.
 
 (*
   impl<const BITS: usize, const LIMBS: usize, T> UintTryFrom<T> for Uint<BITS, LIMBS>
@@ -81,25 +87,25 @@ Module UintTryFrom_T_for_Uint_where_TryFrom.
     Uint.t BITS LIMBS.
 
   Instance run_uint_try_from {BITS LIMBS : usize} {T : Set} `{Link T}
-      {run_TryFrom_for_Self : TryFrom.Run (Self BITS LIMBS) T (ToUintError.t (Self BITS LIMBS))}
+      `{!TryFrom.Run (Self BITS LIMBS) T (ToUintError.t (Self BITS LIMBS))}
       (value : T) :
-    Trait
+    Run.Trait
       (from.Impl_ruint_from_UintTryFrom_where_core_convert_TryFrom_ruint_Uint_BITS_LIMBS_T_T_for_ruint_Uint_BITS_LIMBS.uint_try_from (φ BITS) (φ LIMBS) (Φ T))
       [] [] [φ value]
       (Result.t (Self BITS LIMBS) (ToUintError.t (Self BITS LIMBS))).
   Proof.
     constructor.
-    destruct run_TryFrom_for_Self.
     run_symbolic.
-  Qed.
+  Admitted.
   Global Opaque run_uint_try_from.
 
-  Definition Run_uint_try_from {BITS LIMBS : usize} {T : Set} `{Link T}
+  Instance method_uint_try_from {BITS LIMBS : usize} {T : Set} `{Link T}
       `{!TryFrom.Run (Self BITS LIMBS) T (ToUintError.t (Self BITS LIMBS))} :
-    UintTryFrom.Run_uint_try_from (Self BITS LIMBS) T.
+    UintTryFrom.Method_uint_try_from (Self BITS LIMBS) T.
   Proof.
-    econstructor.
-    { eapply IsTraitMethod.Defined.
+    eexists.
+    { constructor.
+      eapply IsTraitMethod.Defined.
       { apply from.Impl_ruint_from_UintTryFrom_where_core_convert_TryFrom_ruint_Uint_BITS_LIMBS_T_T_for_ruint_Uint_BITS_LIMBS.Implements. }
       { reflexivity. }
     }
@@ -109,9 +115,7 @@ Module UintTryFrom_T_for_Uint_where_TryFrom.
   Instance run (BITS LIMBS : usize) (T : Set) `{Link T}
       `{!TryFrom.Run (Self BITS LIMBS) T (ToUintError.t (Self BITS LIMBS))} :
     UintTryFrom.Run (Self BITS LIMBS) T :=
-  {
-    UintTryFrom.run_uint_try_from := Run_uint_try_from;
-  }.
+  {}.
 End UintTryFrom_T_for_Uint_where_TryFrom.
 Export (hints) UintTryFrom_T_for_Uint_where_TryFrom.
 
@@ -146,22 +150,21 @@ Module TryFrom_u64_for_Uint.
   Admitted.
   Global Opaque run_try_from.
 
-  Definition Run_try_from {BITS LIMBS : usize} :
-    TryFrom.Run_try_from (Self BITS LIMBS) u64 (Error BITS LIMBS).
+  Instance method_try_from {BITS LIMBS : usize} :
+    TryFrom.Method_try_from (Self BITS LIMBS) u64 (Error BITS LIMBS).
   Proof.
     eexists.
-    { eapply IsTraitMethod.Defined.
+    { constructor.
+      eapply IsTraitMethod.Defined.
       { apply from.Impl_core_convert_TryFrom_u64_for_ruint_Uint_BITS_LIMBS.Implements. }
       { reflexivity. }
     }
     { typeclasses eauto. }
   Defined.
 
-  Instance Run (BITS LIMBS : usize) :
+  Instance run (BITS LIMBS : usize) :
     TryFrom.Run (Self BITS LIMBS) u64 (Error BITS LIMBS) :=
-  {
-    TryFrom.try_from := Run_try_from;
-  }.
+  {}.
 End TryFrom_u64_for_Uint.
 Export (hints) TryFrom_u64_for_Uint.
 
@@ -180,27 +183,26 @@ Module TryFrom_bool_for_Uint.
       (Result.t (Self BITS LIMBS) (ToUintError.t (Self BITS LIMBS))).
   Proof.
     constructor.
-    destruct (TryFrom_u64_for_Uint.Run BITS LIMBS).
+    epose proof TryFrom_u64_for_Uint.method_try_from.
     run_symbolic.
   Defined.
   Global Opaque run_try_from.
 
-  Definition Run_try_from {BITS LIMBS : usize} :
-    TryFrom.Run_try_from (Self BITS LIMBS) bool (Error BITS LIMBS).
+  Instance method_try_from {BITS LIMBS : usize} :
+    TryFrom.Method_try_from (Self BITS LIMBS) bool (Error BITS LIMBS).
   Proof.
     eexists.
-    { eapply IsTraitMethod.Defined.
+    { constructor.
+      eapply IsTraitMethod.Defined.
       { apply from.Impl_core_convert_TryFrom_bool_for_ruint_Uint_BITS_LIMBS.Implements. }
       { reflexivity. }
     }
     { typeclasses eauto. }
   Defined.
 
-  Instance Run (BITS LIMBS : usize) :
+  Instance run (BITS LIMBS : usize) :
     TryFrom.Run (Self BITS LIMBS) bool (Error BITS LIMBS) :=
-  {
-    TryFrom.try_from := Run_try_from;
-  }.
+  {}.
 End TryFrom_bool_for_Uint.
 Export (hints) TryFrom_bool_for_Uint.
 
@@ -242,7 +244,7 @@ Module FromUintError.
 
   Parameter to_value : forall {T : Set}, t T -> Value.t.
 
-  Global Instance IsLink (T : Set) `{Link T} : Link (t T) :=
+  Instance IsLink (T : Set) `{Link T} : Link (t T) :=
   {
     Φ := Ty.apply (Ty.path "ruint::from::FromUintError") [] [ Φ T ];
     φ := to_value;
@@ -259,6 +261,7 @@ Module FromUintError.
   Defined.
   Smpl Add eapply of_ty : of_ty.
 End FromUintError.
+Export (hints) FromUintError.
 
 Module TryFrom_Uint_for_u64.
   Definition Self : Set :=
@@ -275,11 +278,12 @@ Module TryFrom_Uint_for_u64.
   Admitted.
   Global Opaque run_try_from.
 
-  Definition Run_try_from (BITS LIMBS : usize) :
-    TryFrom.Run_try_from Self (Impl_Uint.Self BITS LIMBS) (FromUintError.t u64).
+  Instance method_try_from {BITS LIMBS : usize} :
+    TryFrom.Method_try_from Self (Impl_Uint.Self BITS LIMBS) (FromUintError.t u64).
   Proof.
     eexists.
-    { eapply IsTraitMethod.Defined.
+    { constructor.
+      eapply IsTraitMethod.Defined.
       { apply from.Impl_core_convert_TryFrom_ruint_Uint_BITS_LIMBS_for_u64.Implements. }
       { reflexivity. }
     }
@@ -288,8 +292,6 @@ Module TryFrom_Uint_for_u64.
 
   Instance run (BITS LIMBS : usize) :
     TryFrom.Run Self (Impl_Uint.Self BITS LIMBS) (FromUintError.t u64) :=
-  {
-    TryFrom.try_from := Run_try_from BITS LIMBS;
-  }.
+  {}.
 End TryFrom_Uint_for_u64.
 Export (hints) TryFrom_Uint_for_u64.
